\documentclass[10pt]{amsart}
\usepackage[margin=1.4in]{geometry}
\usepackage[usenames,dvipsnames,cmyk]{xcolor} %load first
\usepackage{cancel}
\usepackage{graphicx,subfig}
\usepackage{mathtools}

\graphicspath{ {./images/} }

\usepackage{amssymb,amsmath,enumitem,url}

\newcommand{\D}{\mathrm{d}}
\newcommand{\I}{\mathrm{i}}
\DeclareMathOperator{\E}{e}
\DeclareMathOperator{\OO}{O}
\DeclareMathOperator{\oo}{o}
\DeclareMathOperator{\erfc}{erfc}
\DeclareMathOperator{\real}{Re}
\DeclareMathOperator{\imag}{Im}
\usepackage{tikz}
\usepackage[framemethod=tikz]{mdframed}
\theoremstyle{nonumberplain}

\mdtheorem[innertopmargin=5pt]{lemma}{Lemma}
\mdtheorem[innertopmargin=-5pt]{sol}{Solution}
%\newmdtheoremenv[innertopmargin=-5pt]{sol}{Solution}
\definecolor{MichiganBlue}{HTML}{00274C}
\definecolor{MichiganYellow}{HTML}{FFCB05}  
\definecolor{NicePurple}{RGB}{75,56,76} %PrincePurple
\definecolor{NiceRed}{RGB}{230,37,52}
\definecolor{MidnightBlue}{rgb}{0.1, 0.1, 0.44}
\usepackage[colorlinks=true, linkcolor=MidnightBlue, citecolor=MidnightBlue, urlcolor=MidnightBlue]{hyperref}

\begin{document}
\pagestyle{empty}

\newcommand{\mline}{\vspace{.2in}\hrule\vspace{.2in}}

\noindent
\text{Hunter Lybbert} \\
\text{Student ID: 2426454} \\
\text{12-02-24} \\
\text{AMATH 567} \\

\title{\bf { Homework 10} }


\maketitle
\noindent
Collaborators*: Laura Thomas, Cooper Simpson, Nate Ward, Sophia Kamien \\
\\
\tiny
\text{*Listed in no particular order. And anyone I discussed at least part of one problem with is considered a collaborator.}
\normalsize


\mline
\begin{enumerate}[label={\bf {\arabic*}:}]
\item I sketched the following in class.  Complete the argument.  Show that for an integer $j \in (-N,N)$ and $h > 0$,
\begin{align*}
\lim_{h \to \infty} \int_{\I h}^{\I h + \pi} \frac{\E^{2 \I jz}}{\tan (N z)} \D z
	= \begin{cases} - \I \pi & j = 0,\\ 0 & \text{otherwise}.\end{cases}
\end{align*}
 
\noindent
\textit{Solution:} \\
\textbf{TODO:} \\
Following the sketch provided in class let's look at an import representation of $\tan (Nz)$
\begin{align*}
\tan(N z) &= \frac {\sin (N z)}{\cos (N z)} \\
	&= \frac{ \E^{\I N z} + \E^{- \I N z} }{2\I} \left( \frac {\E^{\I N z} - \E^{- \I N z}} 2 \right)^{-1} \\
	&= \frac{ \E^{\I N z} + \E^{- \I N z} }{2\I} \left( \frac 2 {\E^{\I N z} - \E^{- \I N z}} \right) \\
	&= \frac 1 \I \left( \frac { \E^{\I N z} + \E^{- \I N z} }{ \E^{\I N z} - \E^{- \I N z} } \right) \\
	&= \frac 1 \I \Bigg( \frac {\E^{\I N z}}{\E^{\I N z}} \left( \frac { 1 + \E^{- 2 \I N z} }{ 1 - \E^{- 2 \I N z} } \right) \Bigg) \\
	&= \frac 1 \I \Bigg( \frac { 1 + \E^{- 2 \I N z} }{ 1 - \E^{- 2 \I N z} } \Bigg) \\
	&= \frac 1 \I \Bigg( \frac { 1 + \left( \cos (N z) - \I \sin(N z) \right)^2 }{ 1 - \left( \cos (N z) - \I \sin(N z) \right)^2 } \Bigg) \\
	&= \frac 1 \I \Bigg( \frac { 1 +  \cos^2 (N z) - 2 \I \cos(N z) \sin(N z)- \sin^2(N z) }{ 1 - \cos^2 (N z) + 2 \I \cos(N z) \sin(N z) + \sin^2(N z) } \Bigg) \\
	&... \\
	&= \I + \mathcal O(\E^{-2Nh})
\end{align*}
\newpage

\item From A\&F: 4.2.1 (b) \\
 
\noindent
\textit{Solution:} \\
See solution to problem 2 from homework set 9. \\
\qed \\


\item From A\&F: 4.2.2 (a, h) \\
Evaluate the following real integrals by residue integration: \\
 
\noindent
(a) \\
\begin{align*}
\int_{-\infty}^{\infty} \frac {x \sin x}{x^2 + a^2 } \D x, \quad a^2 > 0
\end{align*}
\textit{Solution:} \\
We can also look at just the imaginary part of another version of this integral
\begin{align*}
\int_{-\infty}^{\infty} \frac {x \sin x}{x^2 + a^2 } \D x
	&= { \rm Im } \int_{-\infty}^{\infty} \frac {x \E^{\I x}}{x^2 + a^2 } \D x \\
	&= { \rm Im } \int_{-\infty}^{\infty} \frac {x \left( \cos x + \I \sin x \right)}{x^2 + a^2 } \D x \\
	&= { \rm Im } \left[
		\int_{-\infty}^{\infty} \frac {x \cos x }{x^2 + a^2 } \D x
		+ \I \int_{-\infty}^{\infty} \frac {x \sin x }{x^2 + a^2 } \D x
	\right] \\
	&= \int_{-\infty}^{\infty} \frac {x \sin x}{x^2 + a^2 } \D x.
\end{align*}
Therefore, we consider the integral 
$$
\int_{-\infty}^{\infty} \frac {x \E^{\I x}}{x^2 + a^2 } \D x
$$
and then take the imaginary part at the end.
In order to evaluate this integral we look at the integral over the contour $C$ which is a counterclockwise semicircle in the upper half plane with radius $R$.
Then applying the Residue Theorem and taking the limit as $R \rightarrow \infty$, we have the following
\begin{align*}
\oint_{C} \frac {z \E^{\I z}}{z^2 + a^2 } \D z
	&= \int_{-R}^{R} \frac {x \E^{\I x}}{x^2 + a^2 } \D x + \oint_{C^{R}} \frac {z \E^{\I z}}{z^2 + a^2 } \D z \\
2 \pi \I\sum_{w \in S} \left( \frac {z \E^{\I z}}{z^2 + a^2 } \right)
	&= \int_{-\infty}^{\infty} \frac {x \E^{\I x}}{x^2 + a^2 } \D x + \cancelto{0}{\oint_{C^{R}} \frac {z \E^{\I z}}{z^2 + a^2 } \D z}
\end{align*}
where $S$ is the set of singularities of our function in the upper half plane and I claim the $C_R$ contour integral goes to 0 by Jordan's Lemma.
I will verify this second claim next.\\

\noindent
To justify using Jordan's Lemma I want to note we are using $k = 1$ in assumptions from the lemma of concern.
Moreover, I will be assuming $a > 0$ for now.
Additionally, we need to show $f(z) \rightarrow 0$ {\bf uniformly} as $R\rightarrow \infty $ in $C_R$, that is if $|f(z)| \leq K_R$, where $K_R$ only depends on $R$ and not arg $z$ and $K_R \rightarrow 0 $ as $ R \rightarrow \infty$.
Let's first find this bound $K_R$
\begin{align*}
|f(z)| &= \left| \frac z {z^2 + a^2} \right| \\
	&= \left| \frac {R \E^{\I \theta}} {R^2 \E^{2 \I \theta} + a^2} \right| \\
	&= \frac {R} { \left|  R^2 \E^{2 \I \theta} + a^2 \right| } \\
	&\leq \frac {R} { \big| \left|R^2 \E^{2 \I \theta} \right| - \left| - a^2 \right| \big| } \\
	&\leq \frac {R} { R^2 - a^2 }.
\end{align*}
In the final two steps with inequalities we first apply the inverse triangle inequality, followed by recognizing the following.
Since $R$ is becoming arbitrarily large then for a given $a$ eventually $R$ will be larger such that $R^2 > a^2$ and therefore the expression $R^2 - a^2 > 0$ thus we can drop the absolute value in the end.
Now, let $K_R = R/(R^2 - a^2)$.
Clearly the denominator will win out as we take $R \rightarrow \infty$ since it has a squared $R$ in it, while the numerator only has a linear $R$.
Therefore, $K_R \rightarrow 0 $ as $ R \rightarrow \infty$ and thus $f(z) \rightarrow 0$ {\bf uniformly} as $R\rightarrow \infty $ in $C_R$.
Thus we have verified that
$$
\cancelto{0}{\oint_{C^{R}} \frac {z \E^{\I z}}{z^2 + a^2 } \D z}
$$
by Jordan's Lemma. \\

\noindent
\textbf{TODO: Square away that this is a good argument or not.} \\
We need to evaluate this limit
$$
\lim_{R \rightarrow \infty} \frac z {z^2 + a^2} = \frac R {R^2 + a^2} = \frac \infty \infty
$$
and then use L'HÃ´pitals to get
$$
\lim_{R \rightarrow \infty} \frac z {z^2 + a^2} = \frac 1 {z} = 0
$$
Therefore we no longer need to be concerned with the integral over $C_R$.
Notice the denominator of our function factors to $(z - \I a)(z + \I a)$ therefore the set of singularities in the upper half plane is $S = \{ \I a \} $.
Hence we have
\begin{align*}
\int_{-\infty}^{\infty} \frac {x \E^{\I x}}{x^2 + a^2 } \D x
	&= 2 \pi \I \sum_{w \in S} \underset{z = w }{ \rm Res } \left( \frac {z \E^{\I z}}{z^2 + a^2 } \right) \\
	&= 2 \pi \I \, \, \underset{z = \I a }{ \rm Res } \left( \frac {z \E^{\I z}}{(z - \I a)(z + \I a) } \right) \\
	&= 2 \pi \I \left( \frac {\I a \E^{\I^2 a}}{ \I a + \I a } \right) \\
	&= 2 \pi \I \left( \frac {\I a \E^{- a}}{ 2 \I a } \right) \\
	&= \pi \I \E^{- a}.
\end{align*}
Therefore,
\begin{align*}
\int_{-\infty}^{\infty} \frac {x \sin x}{x^2 + a^2 } \D x
	&= { \rm Im } \left[ \int_{-\infty}^{\infty} \frac {x \E^{\| x}}{x^2 + a^2 } \D x \right] \\
	&= { \rm Im } \left[ \pi \I \E^{- a} \right] \\
	&= \pi \E^{- a}
\end{align*}
\textbf{TODO: consider doing a case where $a < 0$.} \\


\noindent
(h) \\
\begin{align*}
\int_{0}^{2 \pi} \frac {\D \theta}{ (5 - 3\sin\theta)^2 }
\end{align*}
\textit{Solution:} \\
Let's begin by reverse parameterizing this into a contour integral around the unit circle.
Notice, using the normal parameterization but going the other way we have, $z = \E^{\I \theta}$ and
$$ \D z = \I \E^{\I \theta } \D \theta \implies \frac 1 {\I z} \D z = \D \theta. $$
Additionally, notice,
$$
\sin\theta = \frac {\E^{\I \theta} - \E^{-\I \theta}}{2 \I} = \frac {z - \frac 1 z}{2 \I}.
$$
Hence, our reverse parameterization can get us here (with a little simplification)
\begin{align*}
\int_{0}^{2 \pi} \frac {\D \theta}{ (5 - 3\sin\theta)^2 }
	&= \oint_{\partial B_1(0)} \left(5 - 3 \left( \frac {z - \frac 1 z}{2 \I} \right) \right)^{-2} \frac {\D z}{ \I z } \\
	&= \oint_{\partial B_1(0)} \left(5 - \frac {3z}{2 \I} + \frac 3 {2 \I z} \right)^{-2} \frac {\D z}{ \I z } \\
	&= \oint_{\partial B_1(0)} \left(\frac {10 \I z - 3z^2 + 3}{2 \I z}\right)^{-2} \frac {\D z}{ \I z } \\
	&= \oint_{\partial B_1(0)} \frac {(2 \I z)^2} {\left(10 \I z - 3z^2 + 3\right)^{2}\I z} \D z \\
	&= \oint_{\partial B_1(0)} \frac {4 \I z} {\left(10 \I z - 3z^2 + 3\right)^{2}} \D z.
\end{align*}
Now we need to factor the quadratic in the denominator to determine the singularities of the integrand
\begin{align*}
10 \I z - 3z^2 + 3
	&= (\I - 3 z)(z - 3 \I) \\
	&= - 3 \left(z - \I / 3 \right) \left(z - 3 \I \right).
\end{align*}
Then we have
\begin{align*}
\oint_{\partial B_1(0)} \frac {4 \I z} {\left(10 \I z - 3z^2 + 3\right)^{2}} \D z
	&= \oint_{\partial B_1(0)} \frac {4 \I z} {\left(- 3 \left(z - \I / 3 \right) \left(z - 3 \I \right)\right)^{2}} \D z \\
	&= \oint_{\partial B_1(0)} \frac {4 \I z} {9 (z - \I / 3 )^2 (z - 3 \I )^2} \D z \\
	&= 2 \pi \I \, \, \underset{z = \I/3 }{ \rm Res } \left( \frac {4 \I z} {9 (z - \I / 3 )^2 (z - 3 \I )^2} \right).
\end{align*}
Let's compute the residue at the simple pole with this formula
\begin{align*}
2 \pi \I \, \, \underset{z = \I a }{ \rm Res } \left( \frac {4 \I z} {9 (z - \I / 3 )^2 (z - 3 \I )^2} \right)
	&= 2 \pi \I \, \, \frac 1 {(2 - 1)!} \frac {\D^{2 - 1}}{\D z^{2 - 1}} \left( \cancel{(z - \I / 3 )^2} \frac {4 \I z} {9 \cancel{(z - \I / 3 )^2} (z - 3 \I )^2} \right) \Bigg|_{\I / 3} \\
	&= 2 \pi \I \, \, \frac {\D}{\D z} \left( \frac {4 \I z} {9 (z - 3 \I )^2} \right) \Bigg|_{\I / 3} \\
	&= 2 \pi \I \, \, \left( \frac {4 \I 9 (z - 3 \I )^2 - 4 \I z (9 \cdot 2 (z - 3 \I ))} {9^2 (z - 3 \I )^4} \right) \Bigg|_{\I / 3} \\
	&= 2 \pi \I \, \, \left( \frac {4 \I (z - 3 \I ) - 8 \I z } {9 (z - 3 \I )^3} \right) \Bigg|_{\I / 3} \\
	&= 2 \pi \I \, \, \left( \frac {4 \I z + 12 - 8 \I z } {9 (z - 3 \I )^3} \right) \Bigg|_{\I / 3} \\
	&= 2 \pi \I \, \, \left( \frac {- 4 \I z + 12 } {9 (z - 3 \I )^3} \right) \Bigg|_{\I / 3} \\
	&= 2 \pi \I \, \, \left( \frac {- 4 \I \frac \I 3 + 12 } {9 (\frac \I 3 - 3 \I )^3} \right) \\
	&= 2 \pi \I \, \, \left( \frac {\frac 4 3 + 12 } {9 (\frac {- 8 \I} 3 )^3} \right) \\
	&= 2 \pi \I \, \, \left( \frac {\frac {40} 3 } {9 \frac {(-1)^3 8 \cdot 64 \I^3} {9 \cdot 3} } \right) \\
	&= 2 \pi \I \, \, \left( \frac { 40 } {- 8 \cdot 64 (-1) \I} \right) \\
	&= \pi \, \, \left( \frac { 40 } {8 \cdot 32 } \right) \\
	&= \frac { 5 \pi } { 32 }.
\end{align*}
\qed \\

\newpage

\item
\begin{enumerate}
\item  Show that
$$
\operatorname{Res}_{z=k} f(z) \cot (\pi z)=\frac{1}{\pi} f(k),
$$
provided $f(z)$ is analytic at $z=k, ~~k \in \mathbb{Z}$. \\
 
\noindent
\textit{Solution:} \\
Recall that if $z = z_k$ is a pole of order $N$ of $f(z)\cot \pi z$ then
$$
\underset{z = z_k }{ \rm Res } \left( f(z)\cot \pi z \right)
	= \frac 1 {(N - 1)!} \lim_{z\rightarrow z_k} \frac {\D^{N -1}}{\D z^{N - 1}} \left[(z - z_k)^N f(z)\cot \pi z \right].
$$
Notice, that the only places where our function $f(z)\cot \pi z$ only blows up in the locations where $\tan(\pi z) = 0$, therefore, $\sin \pi z = 0$.
This holds at all the integers $z=k$.
Each $k \in \mathbb Z $ will therefore be a simple pole of $f(z) \cot \pi z$.
Then let's calculate 
\begin{align*}
\underset{z = k }{ \rm Res } \left( f(z)\cot \pi z \right)
	&= \frac 1 {(1 - 1)!} \lim_{z\rightarrow k} \frac {\D^{1-1}}{\D z^{1 - 1}} \left[(z - k)^1 f(z)\cot \pi z \right] \\
	&= \lim_{z\rightarrow k} \left[(z - k) f(z)\cot \pi z \right] \\
	&= \lim_{z\rightarrow k} \left[ \frac {(z - k) f(z)} {\tan \pi z} \right] \\
	&= \frac {(k - k) f(k)} {\tan \pi k} \\
	&= \frac 0 0.
\end{align*}
Using L'HÃ´pital's, we have
\begin{align*}
\lim_{z\rightarrow k} \left[ \frac {(z - k) f(z)} {\tan \pi z} \right]
	&= \lim_{z\rightarrow k} \left[ \frac {\frac{\D}{\D z}(z - k) f(z)} { \frac{\D}{\D z}\tan \pi z} \right] \\
	&= \lim_{z\rightarrow k} \left[ \frac {f(z) + (z - k) f^\prime(z)} { \pi \sec^2 (\pi z)} \right] \\
	&= \frac {f(k) + (k - k) f^\prime(k)} { \pi \sec^2 (\pi k)} \\
	&= \frac 1 \pi ( f(k) + (k - k) f^\prime(k) ) \cos^2 (\pi k) \\
	&= \frac 1 \pi f(k) \cos^2 (\pi k) \\
	&= \frac 1 \pi f(k).
\end{align*}
\qed
\\

\newpage

\item Let $\Gamma_N$ be a square contour, with corners at $(N+1 / 2)( \pm 1 \pm i), N \in \mathbb{Z}^{+}$. Show that
$$
|\cot (\pi z)| \leq 2,
$$
for $z$ on $\Gamma_N$.\\
 
\noindent
\textit{Solution:} \\
Consider the following representation of $\cot \pi z$ with some manipulation
\begin{align*}
| \cot \pi z | = \left| \frac 1 {\tan \pi z} \right| &= \left| \frac {\cos \pi z} {\sin \pi z} \right| \\
	&= \left| \cos \pi z ( \sin \pi z )^{-1} \right| \\
	&= \left| \frac {\E^{\I \pi z} + \E^{-\I \pi z} }{2} \left( \frac {\E^{\I \pi z} - \E^{-\I \pi z} }{2\I} \right)^{-1} \right| \\
	&= \left| \frac {\E^{\I \pi z} + \E^{-\I \pi z} }{2} \left( \frac {2\I} {\E^{\I \pi z} - \E^{-\I \pi z} } \right) \right| \\
	&= \left| \frac {\I \left( \E^{\I \pi z} + \E^{-\I \pi z} \right) } {\E^{\I \pi z} - \E^{-\I \pi z} } \right| \\
	&\leq |\I | \left| \frac { \E^{\I \pi z} + \E^{-\I \pi z} } {\E^{\I \pi z} - \E^{-\I \pi z} } \right| \\
	&= \left| \frac { \E^{\I \pi z} + \E^{-\I \pi z} } {\E^{\I \pi z} - \E^{-\I \pi z} } \right| \\
	&= \left| \frac {\E^{\I \pi z}} {\E^{\I \pi z}} \frac { 1 + \E^{- 2 \pi \I z} } {1 - \E^{-2 \pi \I z} } \right| \\
	&= \left| \frac { 1 + \E^{- 2 \pi \I z} } {1 - \E^{-2 \pi \I z} } \right|.
\end{align*}
We will analyze this to show $|\cot \pi z| \leq 2$ along the contour $\Gamma_N$. \\
\textbf{TODO: Parameterize the contour (along the top and bottom pieces of the rectangle where the real part is parameterized but the imaginary part is constant) to get something in terms of $ \coth \pi z $ and show that that is bounded by 2 since it is a decreasing function.}
\textbf{TODO: Do something similar to this for the sides of the contour where the imaginary part is variable but the real part is constant.}
\begin{align*}
f(x) = mx + b
\end{align*}


\item Suppose $f(z)=p(z) / q(z)$, where $p(z)$ and $q(z)$ are polynomials, so that the degree of $q(z)$ is at least two more than the degree of $p(z)$. Show that
$$
\lim _{N \rightarrow \infty}\left|\oint_{\Gamma_N} \frac{p(z)}{q(z)} \cot (\pi z) d z\right|=0
$$
 
\noindent
\textit{Solution:} \\
\textbf{TODO:}
\begin{align*}
f(x) = mx + b
\end{align*}


\item Suppose, in addition, that $q(z)$ has no roots at the integers. Show that
$$
\sum_{k=-\infty}^{\infty} \frac{p(k)}{q(k)}=-\pi \sum_j \operatorname{Res}_{z=z_j} f(z) \cot (\pi z)
$$
where the $z_j$'s are the roots of $q(z)$. Notice that the sum on the
right-hand side has a finite number of terms. \\
 
\noindent
\textit{Solution:} \\
\textbf{TODO:}
\begin{align*}
f(x) = mx + b
\end{align*}

\newpage

\item Use the result of the previous problem to evaluate the following sums:
\begin{enumerate}
\item  $\displaystyle \sum_{k=-\infty}^{\infty} \frac{1}{k^2+1}$ \\
 
\noindent
\textit{Solution:} \\
\textbf{TODO:}
\begin{align*}
f(x) = mx + b
\end{align*}

\item  $\displaystyle \sum_{k=-\infty}^{\infty} \frac{1}{k^4+1}$ \\
 
\noindent
\textit{Solution:} \\
\textbf{TODO:}
\begin{align*}
f(x) = mx + b
\end{align*}


\item  $\displaystyle \sum_{k=-\infty}^{\infty} \frac{1}{k^2-1/4}$ \\
 
\noindent
\textit{Solution:} \\
\textbf{TODO:}
\begin{align*}
f(x) = mx + b
\end{align*}


\item  $\displaystyle \sum_{k=-\infty}^{\infty} \frac{1}{16k^4 -1}$ \\
 
\noindent
\textit{Solution:} \\
\textbf{TODO:}
\begin{align*}
f(x) = mx + b
\end{align*}


\end{enumerate}
\end{enumerate}

\end{enumerate}
  
\end{document}

%%% Local Variables:
%%% mode: latex
%%% TeX-master: t
%%% End:
